Lean4Lean/Theory/Typing/Basic.lean
@@ -1,0 +1,76 @@
+import Lean4Lean.Theory.VEnv
+
+namespace Lean4Lean
+
+inductive Lookup : List VExpr → Nat → VExpr → Prop where
+  | zero : Lookup (ty::Γ) 0 ty.lift
+  | succ : Lookup Γ n ty → Lookup (A::Γ) (n+1) ty.lift
+
+namespace VEnv
+
+inductive Judgment where
+  | hasType (e A : VExpr)
+  | defeq (e1 e2 A : VExpr)
+
+section
+set_option hygiene false
+local notation:65 Γ " ⊢ " e " : " A:30 => IsDefEq Γ e e A
+local notation:65 Γ " ⊢ " e1 " ≡ " e2 " : " A:30 => IsDefEq Γ e1 e2 A
+variable (env : VEnv) (uvars : Nat)
+
+inductive IsDefEq : List VExpr → VExpr → VExpr → VExpr → Prop where
+  | bvar : Lookup Γ i A → Γ ⊢ .bvar i : A
+  | const :
+    env.constants c = some (some ci) →
+    (∀ l ∈ ls, l.WF uvars) →
+    ls.length = ci.uvars →
+    Γ ⊢ .const c ls : ci.type.instL ls
+  | symm : Γ ⊢ e ≡ e' : A → Γ ⊢ e' ≡ e : A
+  | trans : Γ ⊢ e₁ ≡ e₂ : A → Γ ⊢ e₂ ≡ e₃ : A → Γ ⊢ e₁ ≡ e₃ : A
+  | sortDF :
+    l.WF uvars → l'.WF uvars → l ≈ l' →
+    Γ ⊢ .sort l ≡ .sort l' : .sort (.succ l)
+  | appDF :
+    Γ ⊢ f ≡ f' : .forallE A B →
+    Γ ⊢ a ≡ a' : A →
+    Γ ⊢ .app f a ≡ .app f' a' : B.inst a
+  | lamDF :
+    Γ ⊢ A ≡ A' : .sort u →
+    A::Γ ⊢ body ≡ body' : B →
+    Γ ⊢ .lam A body ≡ .lam A' body' : .forallE A B
+  | forallEDF :
+    Γ ⊢ A ≡ A' : .sort u →
+    A::Γ ⊢ body ≡ body' : .sort v →
+    Γ ⊢ .forallE A body ≡ .forallE A' body' : .sort (.imax u v)
+  | defeqDF : Γ ⊢ A ≡ B : .sort u → Γ ⊢ e1 ≡ e2 : A → Γ ⊢ e1 ≡ e2 : B
+  | beta :
+    A::Γ ⊢ e : B → Γ ⊢ e' : A →
+    Γ ⊢ .app (.lam A e) e' ≡ e.inst e' : B.inst e'
+  | eta :
+    Γ ⊢ e : .forallE A B →
+    Γ ⊢ .lam A (.app e.lift (.bvar 0)) ≡ e : .forallE A B
+  | proofIrrel :
+    Γ ⊢ p : .sort .zero → Γ ⊢ h : p → Γ ⊢ h' : p →
+    Γ ⊢ h ≡ h' : p
+  | extra :
+    env.defeqs df → (∀ l ∈ ls, l.WF uvars) → ls.length = df.uvars →
+    Γ ⊢ df.lhs.instL ls ≡ df.rhs.instL ls : df.type.instL ls
+
+end
+
+def HasType (env : VEnv) (U : Nat) (Γ : List VExpr) (e A : VExpr) : Prop :=
+  IsDefEq env U Γ e e A
+
+def IsType (env : VEnv) (U : Nat) (Γ : List VExpr) (A : VExpr) : Prop :=
+  ∃ u, env.HasType U Γ A (.sort u)
+
+def CtxWF (env : VEnv) (U : Nat) : List VExpr → Prop
+  | [] => True
+  | A::Γ => CtxWF env U Γ ∧ IsType env U Γ A
+
+end VEnv
+
+def VConstant.WF (env : VEnv) (ci : VConstant) : Prop := env.IsType ci.uvars [] ci.type
+
+def VDefEq.WF (env : VEnv) (df : VDefEq) : Prop :=
+  env.HasType df.uvars [] df.lhs df.type ∧ env.HasType df.uvars [] df.rhs df.type
