Lean4Lean/Theory/VLevel.lean
@@ -51,8 +51,14 @@ protected def Equiv (a b : VLevel) : Prop := a.eval = b.eval
 
 instance : HasEquiv VLevel := ⟨VLevel.Equiv⟩
 
+theorem equiv_def' {a b : VLevel} : a ≈ b ↔ a.eval = b.eval := .rfl
+theorem equiv_def {a b : VLevel} : a ≈ b ↔ ∀ ls, a.eval ls = b.eval ls := funext_iff
+
 theorem le_antisymm_iff {a b : VLevel} : a ≈ b ↔ a ≤ b ∧ b ≤ a :=
-  funext_iff.trans <| (forall_congr' fun _ => Nat.le_antisymm_iff).trans forall_and
+  equiv_def.trans <| (forall_congr' fun _ => Nat.le_antisymm_iff).trans forall_and
+
+theorem succ_congr {a b : VLevel} (h : a ≈ b) : VLevel.succ a ≈ .succ b := by
+  simpa [equiv_def, eval] using h
 
 theorem toLevel_inj {ls : List Name} (d : ls.Nodup)
     {l₁ l₂ : VLevel} (eq : l₁.toLevel ls = l₂.toLevel ls) : l₁ = l₂ := sorry
@@ -64,6 +70,36 @@ def inst : VLevel → VLevel
   | .max l₁ l₂ => .max l₁.inst l₂.inst
   | .imax l₁ l₂ => .imax l₁.inst l₂.inst
   | .param i => ls.getD i .zero
+
+theorem inst_inst {l : VLevel} : (l.inst ls).inst ls' = l.inst (ls.map (VLevel.inst ls')) := by
+  induction l <;> simp [inst, *, List.getD_eq_get?]
+  case param n => cases ls.get? n <;> simp [inst]
+
+theorem eval_inst {l : VLevel} : (l.inst ls).eval ns = l.eval (ls.map (VLevel.eval ns)) := by
+  induction l <;> simp [eval, inst, *, List.getD_eq_get?]
+  case param n => cases ls.get? n <;> simp [eval]
+
+theorem WF.inst {l : VLevel} (H : ∀ l ∈ ls, l.WF n) : (l.inst ls).WF n := by
+  induction l with
+  | zero => trivial
+  | succ _ ih => exact ih
+  | max _ _ ih1 ih2 | imax _ _ ih1 ih2 => exact ⟨ih1, ih2⟩
+  | param i =>
+    simp [VLevel.inst, List.getD_eq_get?]
+    cases e : ls.get? i with
+    | none => trivial
+    | some => exact H _ (List.get?_mem e)
+
+theorem inst_congr {l : VLevel} (h1 : l ≈ l') (h2 : List.Forall₂ (·≈·) ls ls') :
+    l.inst ls ≈ l'.inst ls' := by
+  simp [equiv_def, eval_inst, ← equiv_def.1 h1]
+  intro ns; congr 1
+  induction h2 with
+  | nil => rfl
+  | cons h2 => simp [*, equiv_def.1 h2]
+
+theorem inst_congr_l {l : VLevel} (h1 : l ≈ l') : l.inst ls ≈ l'.inst ls :=
+  inst_congr h1 <| .rfl fun _ _ => rfl
 
 variable (ls : List Name) in
 def ofLevel : Level → Option VLevel
